---
published: true
---

These equations work properly:
```
\\[ \frac{1}{n^{2}} \\]

\\[ J(\theta) = \frac{1}{2m}[\sum_{i=1}^m(h_\theta (x^{(i)}) - y^{(i)})^2 + \lambda\sum_{j=1}^n\theta^2_j] \\]
```

\\[ \frac{1}{n^{2}} \\]

\\[ J(\theta) = \frac{1}{2m}[\sum_{i=1}^m(h_\theta (x^{(i)}) - y^{(i)})^2 + \lambda\sum_{j=1}^n\theta^2_j] \\]

This one doesn't work:
```
\\[ F'(\theta_*)=\lim\limits_{\theta\to\theta_*}\frac{F(\theta)-F(\theta_*)}{\theta-\theta_*} \\]
```
\\[ F'(\theta_*)=\lim\limits_{\theta\to\theta_*}\frac{F(\theta)-F(\theta_*)}{\theta-\theta_*} \\]
